MxDH: add flexibility to postcondition_norets so loops can consider local variable state, and continue progress on montladder compilation

src/Examples/ECC/DownTo.v
@@ -1,12 +1,12 @@
 Require Import Rupicola.Lib.Api.
 
 Section Gallina.
-  Definition foreach_nat
-             {state} init nats (step:state->nat->state) : state :=
-    fold_left step nats init.
+  Definition downto'
+             {state} init start count (step:state->nat->state) : state :=
+    fold_left step (rev (skipn start (seq 0 count))) init.
   Definition downto
              {state} init count (step:state->nat->state) : state :=
-    foreach_nat init (seq 0 count) step.
+    downto' init 0 count step.
 End Gallina.
 
 Section Compile.
@@ -21,13 +21,22 @@ Section Compile.
            | H : word.unsigned ?x = _
              |- context [word.sub ?x (word.of_Z _)] =>
              rewrite <-(word.of_Z_unsigned x); rewrite H
+           | H : forall l i,
+               map.get (_ l i) ?x = map.get l ?x |- _ =>
+             rewrite H
+           | |- context [S (?x - 1)] =>
+             replace (S (x-1)) with x by lia
            | _ => progress subst_lets_in_goal
            | _ => progress change 1%Z with (Z.of_nat 1)
            | _ => rewrite map.get_put_same by auto
            | _ => rewrite <-word.ring_morph_sub
            | _ => rewrite <-Nat2Z.inj_sub by lia
            | _ => reflexivity
-           | _ => solve [eauto]
+           | _ => lazymatch goal with
+                  | |- (_ < _)%nat => lia
+                  | |- (_ <= _)%nat => lia
+                  | _ => solve [eauto]
+                  end
            end.
 
   Local Ltac use_cmd_hyp :=
@@ -62,155 +71,11 @@ Section Compile.
     reflexivity.
   Qed.
 
-  (* TODO : move *)
-  Lemma hd_map {A B} (f : A -> B) (x : A) l :
-    hd (f x) (List.map f l) = f (hd x l).
-  Proof. destruct l; reflexivity. Qed.
-
-  Lemma compile_foreach_nat :
-    forall (locals: Semantics.locals) (mem: Semantics.mem)
-           (locals_ok : Semantics.locals -> Prop)
-      tr R R' functions T (pred: T -> _ -> Prop)
-      {state} (init : state) ns ws step step_impl k k_impl i_var
-      (step_locals : Semantics.locals -> nat -> Semantics.locals)
-      (State : Semantics.locals -> state -> Semantics.mem -> Prop),
-      (State (map.put locals i_var (hd (word.of_Z 0) ws)) init * R')%sep mem ->
-      ns = List.map Z.to_nat (List.map word.unsigned ws) ->
-      let v := foreach_nat init ns step in
-      (let head := v in
-       (* loop iteration case *)
-       forall tr l li m st i,
-         let wi := word.of_Z (Z.of_nat i) in
-         (State l st * R')%sep m ->
-         l = foreach_nat locals (firstn i ns) step_locals ->
-         li = map.put l i_var wi ->
-         find step_impl
-         implementing (State (step_locals l i) (step st i))
-         and-locals-post (eq (step_locals l i))
-         with-locals li and-memory m and-trace tr and-rest R
-         and-functions functions) ->
-      (let head := v in
-       (* post-loop case *)
-       forall tr l m,
-         (State l head * R')%sep m ->
-         l = foreach_nat locals ns step_locals ->
-         find k_impl
-         implementing (pred (k head))
-         and-locals-post locals_ok
-         with-locals l and-memory m and-trace tr and-rest R
-         and-functions functions) ->
-      (let head := v in
-       (* while (i = n; 0 < i; pass)
-          { i--; step i } *)
-       find (cmd.seq
-               (cmd.seq
-                  (cmd.set i_var (expr.literal (Z.of_nat (hd 0 ns))))
-                  (cmd.while
-                     (expr.op bopname.ltu
-                              (expr.literal 0) (expr.var i_var))
-                     (cmd.seq
-                        (cmd.set i_var
-                                 (expr.op bopname.sub
-                                          (expr.var i_var)
-                                          (expr.literal 1)))
-                        step_impl)))
-               k_impl)
-       implementing (pred (dlet head k))
-       and-locals-post locals_ok
-       with-locals locals and-memory mem and-trace tr and-rest R
-       and-functions functions).
+  Lemma downto'_step {A} i count (step :A -> _) init :
+    0 < i <= count ->
+    step (downto' init i count step) (i-1) = downto' init (i-1) count step.
   Proof.
-    repeat straightline'.
-
-    (* handle while *)
-    WeakestPrecondition.unfold1_cmd_goal;
-      (cbv beta match delta [WeakestPrecondition.cmd_body]).
-    exists nat, lt.
-    exists (fun i t m l =>
-              let st :=
-                  foreach_nat init (firstn i ns) step in
-              (State l st * R')%sep m
-              /\ tr = t
-              /\ (exists wi,
-                     word.unsigned wi = Z.of_nat i
-                     /\ map.get l i_var = Some wi)).
-    ssplit; eauto using lt_wf; [ | ].
-
-    { cbv zeta.
-      exists (hd (Z.to_nat (word.unsigned (word.of_Z 0))) ns);
-        subst ns; ssplit;
-        [ | | | exists (hd (word.of_Z 0) ws)];
-        repeat match goal with
-               | _ => rewrite hd_map
-               | _ => rewrite map.put_put_same by auto
-               | _ => rewrite map.get_put_same by auto
-               | _ => rewrite word.of_Z_unsigned
-               | _ => rewrite skipn_all2 by (rewrite seq_length; lia)
-               | _ => progress subst_lets_in_goal
-               | _ => progress cbn [rev]
-               | _ => solve [eauto]
-               end.
-      { replace (hd 0) with (hd (Z.to_nat (word.unsigned (word.of_Z 0)))).
-      rewrite hd_map.
-      Search List.hd List.map.
-      Search hd List.map.
-
-    }
-
-    { intros. cleanup.
-      repeat straightline'.
-      lazymatch goal with x := context [word.ltu] |- _ => subst x end.
-      rewrite word.unsigned_ltu, word.unsigned_of_Z_0.
-      match goal with
-      | H1 : ?y = Z.of_nat ?x, H2 : 0 < ?x |- _ =>
-        assert (0 < y)%Z by
-            (rewrite H1; change 0%Z with (Z.of_nat 0);
-             apply Nat2Z.inj_lt; auto)
-      end.
-      destruct_one_match;
-        rewrite ?word.unsigned_of_Z_0, ?word.unsigned_of_Z_1;
-        ssplit; try lia; [ | ].
-      { repeat straightline'.
-        use_cmd_hyp; [ | try solve [handle_downto_locals] .. ].
-        2:{
-          Search l.
-          Search l0.
-          subst l0.
-        cleanup; subst.
-        lazymatch goal with
-        | H : word.unsigned ?w = Z.of_nat ?x
-          |- exists i : nat, _ /\ i < ?x =>
-          exists (x-1)%nat; ssplit;
-            lazymatch goal with
-            | |- exists _, _ => exists (word.sub w (word.of_Z 1))
-            | |- sep _ _ _ =>
-              rewrite <-fold_left_skipn_seq by lia; assumption
-            | _ => auto; try lia
-            end
-        end; [ ].
-        ssplit; handle_downto_locals; [ ].
-        rewrite word.unsigned_of_Z.
-        lazymatch goal with
-        | H : word.unsigned ?w = Z.of_nat ?i
-          |- word.wrap (Z.of_nat (?i - 1)) = Z.of_nat (?i - 1) =>
-          pose proof (word.unsigned_range w);
-            apply Z.mod_small; rewrite Nat2Z.inj_sub, <-H by lia
-        end.
-        lia. }
-      { repeat straightline'.
-        match goal with
-        | H : (word.unsigned ?x <= 0)%Z |- _ =>
-          let H' := fresh in
-          assert (word.unsigned x = 0%Z) as H'
-              by (pose proof word.unsigned_range x; lia)
-        end.
-        match goal with
-        | H : context [skipn ?i] |- _ =>
-          replace i with 0 in H by lia; cbn [skipn] in H
-        end.
-        use_cmd_hyp.
-        { eauto. }
-        { subst_lets_in_goal. assumption. } } }
+    cbv [downto']; apply fold_left_skipn_seq.
   Qed.
 
   Locate "implementing".
@@ -223,27 +88,35 @@ Section Compile.
       {state} (init : state) count wcount step step_impl k k_impl i_var
       (step_locals : Semantics.locals -> nat -> Semantics.locals)
       (State : Semantics.locals -> state -> Semantics.mem -> Prop),
-      (State (map.put locals i_var wcount) init * R')%sep mem ->
+      let start_locals := map.put locals i_var wcount in
+      let step_locals' :=
+          fun l i =>
+            step_locals (map.put l i_var (word.of_Z (Z.of_nat i))) i in
+      (* step_locals doesn't change i *)
+      (forall l i,
+          map.get (step_locals l i) i_var = map.get l i_var) ->
+      (State start_locals init * R')%sep mem ->
       word.unsigned wcount = Z.of_nat count ->
       0 < count ->
       let v := downto init count step in
       (let head := v in
        (* loop iteration case *)
-       forall tr l li m st i,
-         let wi := word.of_Z (Z.of_nat i) in
+       forall tr l m st i wi,
+         let li := map.put l i_var wi in
+         wi = word.of_Z (Z.of_nat i) ->
          (State l st * R')%sep m ->
-         l = downto' locals i count step_locals ->
-         li = map.put l i_var wi ->
+         l = downto' start_locals (S i) count step_locals' ->
+         i < count ->
          find step_impl
-         implementing (State (step_locals l i) (step st i))
-         and-locals-post (eq (step_locals l i))
-         with-locals li and-memory m and-trace tr and-rest R
+         implementing (State (step_locals li i) (step st i))
+         and-locals-post (eq (step_locals li i))
+         with-locals li and-memory m and-trace tr and-rest R'
          and-functions functions) ->
       (let head := v in
        (* post-loop case *)
        forall tr l m,
          (State l head * R')%sep m ->
-         l = downto locals count step_locals ->
+         l = downto start_locals count step_locals' ->
          find k_impl
          implementing (pred (k head))
          and-locals-post locals_ok
@@ -277,18 +150,18 @@ Section Compile.
       (cbv beta match delta [WeakestPrecondition.cmd_body]).
     exists nat, lt.
     exists (fun i t m l =>
-              let st :=
-                  fold_left step (rev (skipn i (seq 0 count))) init in
+              let st := downto' init i count step in
               (State l st * R')%sep m
               /\ i <= count
               /\ tr = t
+              /\ l = downto' start_locals i count step_locals'
               /\ (exists wi,
                      word.unsigned wi = Z.of_nat i
                      /\ map.get l i_var = Some wi)).
     ssplit; eauto using lt_wf; [ | ].
 
     { cbv zeta.
-      exists count; ssplit; [ | | | exists wcount];
+      exists count; ssplit; [ | | | | exists wcount];
         repeat match goal with
                | H : _ = Z.of_nat count |- _ => rewrite <-H
                | _ => rewrite map.put_put_same by auto
@@ -296,7 +169,8 @@ Section Compile.
                | _ => rewrite word.of_Z_unsigned
                | _ => rewrite skipn_all2 by (rewrite seq_length; lia)
                | _ => progress subst_lets_in_goal
-               | _ => progress cbn [rev]
+               | _ => progress cbn [rev fold_left]
+               | _ => progress cbv [downto']
                | _ => solve [eauto]
                end. }
 
@@ -314,21 +188,20 @@ Section Compile.
         rewrite ?word.unsigned_of_Z_0, ?word.unsigned_of_Z_1;
         ssplit; try lia; [ | ].
       { repeat straightline'.
-        use_cmd_hyp; [ | try solve [handle_downto_locals] .. ].
-        2:{
-          Search l.
-          Search l0.
-          subst l0.
-        cleanup; subst.
+        use_cmd_hyp;
+          [ | try solve [handle_downto_locals] .. ];
+          [ | solve [handle_downto_locals] .. ];
+        cbv [postcondition_norets postcondition_for] in *;
+          cleanup; subst.
         lazymatch goal with
         | H : word.unsigned ?w = Z.of_nat ?x
           |- exists i : nat, _ /\ i < ?x =>
           exists (x-1)%nat; ssplit;
+            rewrite <-?downto'_step by lia;
             lazymatch goal with
             | |- exists _, _ => exists (word.sub w (word.of_Z 1))
-            | |- sep _ _ _ =>
-              rewrite <-fold_left_skipn_seq by lia; assumption
-            | _ => auto; try lia
+            | |- sep _ _ _ => ecancel_assumption
+            | _ => auto; try lia; try solve [handle_downto_locals]
             end
         end; [ ].
         ssplit; handle_downto_locals; [ ].
@@ -347,13 +220,12 @@ Section Compile.
           assert (word.unsigned x = 0%Z) as H'
               by (pose proof word.unsigned_range x; lia)
         end.
-        match goal with
-        | H : context [skipn ?i] |- _ =>
-          replace i with 0 in H by lia; cbn [skipn] in H
-        end.
-        use_cmd_hyp.
-        { eauto. }
-        { subst_lets_in_goal. assumption. } } }
+        use_cmd_hyp;
+          subst_lets_in_goal;
+          match goal with
+          | H : context [downto' _ ?i] |- _ =>
+            replace i with 0 in * by lia
+          end; eauto. } }
   Qed.
 
 End Compile.
