src/Examples/KVStore/Automated.v
@@ -245,6 +245,7 @@ Section KVSwap.
 
   Lemma compile_map_get :
     forall (locals: Semantics.locals) (mem: Semantics.mem)
+           (locals_ok : Semantics.locals -> Prop)
            tr R R' functions T (pred: T -> _ -> Prop)
            m m_ptr m_var M
            k k_ptr k_var
@@ -264,6 +265,7 @@ Section KVSwap.
           (AnnotatedMap m_ptr M * Key k_ptr k * R')%sep mem' ->
           find default_impl
           implementing (pred default)
+          and-locals-post locals_ok
           with-locals (map.put (map.put locals err (word.of_Z 1))
                             var garbage)
           and-memory mem' and-trace tr and-rest R
@@ -276,6 +278,7 @@ Section KVSwap.
            * Key k_ptr k * R')%sep mem' ->
           find K_impl
           implementing (pred (K head))
+          and-locals-post locals_ok
           with-locals (map.put (map.put locals err (word.of_Z 0))
                             var hd_ptr)
           and-memory mem' and-trace tr and-rest R
@@ -287,6 +290,7 @@ Section KVSwap.
                          K_impl
                          default_impl))
        implementing (pred (do_or_default head K default))
+       and-locals-post locals_ok
        with-locals locals and-memory mem and-trace tr and-rest R
        and-functions functions).
   Proof.
@@ -397,6 +401,7 @@ Section KVSwap.
 
   Lemma compile_map_put_replace :
     forall (locals: Semantics.locals) (mem: Semantics.mem)
+           (locals_ok : Semantics.locals -> Prop)
            tr R R' functions T (pred: T -> _ -> Prop)
            m m_ptr m_var M
            k k_ptr k_var
@@ -416,6 +421,7 @@ Section KVSwap.
           * Key k_ptr k * R')%sep mem' ->
          find K_impl
          implementing (pred (K head))
+         and-locals-post locals_ok
          with-locals locals
          and-memory mem' and-trace tr and-rest R
          and-functions functions) ->
@@ -426,6 +432,7 @@ Section KVSwap.
                          [expr.var m_var; expr.var k_var; expr.var v_var])
                K_impl)
        implementing (pred (dlet head K))
+       and-locals-post locals_ok
        with-locals locals and-memory mem and-trace tr and-rest R
        and-functions functions).
   Proof.
