src/Examples/Ttl/Ttl.v
@@ -44,6 +44,7 @@ Section with_semantics.
 
   Lemma compile_nth :
     forall (locals: Semantics.locals) (mem: Semantics.mem)
+           (locals_ok : Semantics.locals -> Prop)
       tr R R' functions T (pred: T -> _ -> Prop)
       {n} (vector: Vector.t Semantics.word n) vector_ptr vector_var
       offset var k k_impl,
@@ -57,6 +58,7 @@ Section with_semantics.
          sep (WordVector vector_ptr vector) R' m ->
          (find k_impl
           implementing (pred (k head))
+          and-locals-post locals_ok
           with-locals (map.put locals var head)
           and-memory m and-trace tr and-rest R
           and-functions functions)) ->
@@ -70,6 +72,7 @@ Section with_semantics.
                                     (expr.literal ((word.unsigned (word.of_Z 8) * Z.of_nat noffset))))))
                      k_impl)
        implementing (pred (dlet head k))
+       and-locals-post locals_ok
        with-locals locals and-memory mem and-trace tr and-rest R
        and-functions functions).
   Proof.
@@ -102,6 +105,7 @@ Section with_semantics.
 
   Lemma compile_replace :
     forall (locals: Semantics.locals) (mem: Semantics.mem)
+           (locals_ok : Semantics.locals -> Prop)
       tr R R' functions T (pred: T -> _ -> Prop)
       {n} (vector: Vector.t Semantics.word n) vector_ptr vector_var
       value value_var offset
@@ -117,6 +121,7 @@ Section with_semantics.
          sep (WordVector vector_ptr head) R' m ->
          (find k_impl
           implementing (pred (k head))
+          and-locals-post locals_ok
           with-locals locals
           and-memory m and-trace tr and-rest R
           and-functions functions)) ->
@@ -128,6 +133,7 @@ Section with_semantics.
                                 (expr.var value_var))
                      k_impl)
        implementing (pred (dlet head k))
+       and-locals-post locals_ok
        with-locals locals and-memory mem and-trace tr and-rest R
        and-functions functions).
   Proof.
